Phi_Semantics/PhiSem_Basic_Control_Flow.thy
@@ -1,0 +1,186 @@
+chapter \<open>Basic Control Flow\<close>
+
+theory PhiSem_Basic_Control_Flow
+  imports PhiSem_Generic_Boolean
+begin
+
+section \<open>Instructions\<close>
+
+paragraph \<open>Non-Branching Selection\<close>
+
+definition op_sel :: "TY \<Rightarrow> (VAL \<times> VAL \<times> VAL, VAL) proc'"
+  where "op_sel TY =
+    \<phi>M_caseV (\<lambda>vc. \<phi>M_caseV (\<lambda>va vb.
+    \<phi>M_getV bool V_bool.dest vc (\<lambda>c.
+    \<phi>M_getV TY id va (\<lambda>a.
+    \<phi>M_getV TY id vb (\<lambda>b.
+    Return (sem_value (if c then b else a)))))))"
+
+paragraph \<open>Branch\<close>
+
+definition op_if :: "'ret proc
+                  \<Rightarrow> 'ret proc
+                  \<Rightarrow> (VAL,'ret) proc'"
+  where "op_if brT brF v =
+    \<phi>M_getV bool V_bool.dest v (\<lambda>c. (if c then brT else brF))"
+
+paragraph \<open>While Loop\<close>
+
+inductive SemDoWhile :: "VAL proc \<Rightarrow> resource \<Rightarrow> unit state \<Rightarrow> bool" where
+  "Success (sem_value (V_bool.mk False)) res \<in> f s \<Longrightarrow> SemDoWhile f s (Success (sem_value ()) res)"
+| "Success (sem_value (V_bool.mk True)) res \<in> f s \<Longrightarrow> SemDoWhile f res s'' \<Longrightarrow> SemDoWhile f s s''"
+| "Exception v e \<in> f s \<Longrightarrow> SemDoWhile f s (Exception v e)"
+| "PartialCorrect \<in> f s \<Longrightarrow> SemDoWhile f s PartialCorrect"
+| "Invalid \<in> f s \<Longrightarrow> SemDoWhile f s Invalid"
+
+lemma "\<nexists> y. SemDoWhile ((\<lambda>res. Return (sem_value (V_bool.mk True)) res) :: VAL proc) res y"
+  apply rule apply (elim exE) subgoal for y
+    apply (induct "((\<lambda>res. Return (sem_value (V_bool.mk True)) (res::resource)) :: VAL proc)" res y
+           rule: SemDoWhile.induct)
+       apply (simp_all add: Return_def det_lift_def) . .
+
+definition op_do_while :: " VAL proc \<Rightarrow> unit proc"
+  where "op_do_while f s = Collect (SemDoWhile f s)"
+
+(* lemma SemDoWhile_deterministic:
+  assumes "SemDoWhile c s s1"
+      and "SemDoWhile c s s2"
+    shows "s1 = s2"
+proof -
+  have "SemDoWhile c s s1 \<Longrightarrow> (\<forall>s2. SemDoWhile c s s2 \<longrightarrow> s1 = s2)"
+    apply (induct rule: SemDoWhile.induct)
+    by (subst SemDoWhile.simps, simp)+
+  thus ?thesis
+    using assms by simp
+qed
+
+lemma SemDoWhile_deterministic2:
+    "SemDoWhile body s x \<Longrightarrow> The ( SemDoWhile body s) = x"
+  using SemDoWhile_deterministic by blast *)
+
+
+paragraph \<open>Recursion\<close>
+
+inductive SemRec :: "(('a,'a) proc' \<Rightarrow> ('a,'a) proc')
+            \<Rightarrow> 'a sem_value \<Rightarrow> resource \<Rightarrow> 'a state set \<Rightarrow> bool"
+where
+  SemRec_I0: "(\<And>g. F g x res = y) \<Longrightarrow> SemRec F x res y"
+| SemRec_IS: "SemRec (F o F) x res y \<Longrightarrow> SemRec F x res y"
+
+definition op_recursion :: "TY list \<Rightarrow> TY list
+                         \<Rightarrow> (('a,'a) proc' \<Rightarrow> ('a,'a) proc')
+                         \<Rightarrow> ('a,'a) proc'"
+  where "op_recursion _ _ F x s = (if (\<exists>t. SemRec F x s t) then The (SemRec F x s) else {})"
+
+section \<open>Abstraction of Procedures\<close>
+
+subsubsection \<open>Syntax for Annotations\<close>
+
+consts Invariant :: \<open>bool \<Rightarrow> bool\<close> ("Inv: _" [37] 36)
+consts Guard :: \<open>bool \<Rightarrow> bool\<close> ("Guard: _" [37] 36)
+
+subsection \<open>Branch-like\<close>
+
+lemma op_sel_\<phi>app:
+  \<open> \<phi>SemType (a \<Ztypecolon> A) TY
+\<Longrightarrow> \<phi>SemType (b \<Ztypecolon> B) TY
+\<Longrightarrow> \<^bold>p\<^bold>r\<^bold>o\<^bold>c op_sel TY (\<phi>V_pair rawc (\<phi>V_pair rawb rawa)) \<lbrace>
+        a \<Ztypecolon> \<^bold>v\<^bold>a\<^bold>l[rawa] A\<heavy_comma> b \<Ztypecolon> \<^bold>v\<^bold>a\<^bold>l[rawb] B\<heavy_comma> c \<Ztypecolon> \<^bold>v\<^bold>a\<^bold>l[rawc] \<bool>
+    \<longmapsto> (if c then a else b) \<Ztypecolon> \<^bold>v\<^bold>a\<^bold>l (if c then A else B)
+    \<rbrace>\<close>
+  unfolding op_sel_def
+  by (cases rawc; cases rawb; cases rawa; cases c; simp add: \<phi>SemType_def subset_iff,
+      rule, rule, rule, simp add: \<phi>expns WT_bool, blast, rule, simp add: \<phi>expns WT_bool, rule,
+      simp add: \<phi>expns WT_bool, rule, simp add: \<phi>expns WT_bool)
+
+lemma branch_\<phi>app:
+  \<open> (\<^bold>p\<^bold>r\<^bold>e\<^bold>m\<^bold>i\<^bold>s\<^bold>e   C \<longrightarrow> \<^bold>p\<^bold>r\<^bold>o\<^bold>c br\<^sub>T \<lbrace> X \<longmapsto> Y\<^sub>T \<^bold>t\<^bold>h\<^bold>r\<^bold>o\<^bold>w\<^bold>s E\<^sub>T \<rbrace>)
+\<Longrightarrow> (\<^bold>p\<^bold>r\<^bold>e\<^bold>m\<^bold>i\<^bold>s\<^bold>e \<not> C \<longrightarrow> \<^bold>p\<^bold>r\<^bold>o\<^bold>c br\<^sub>F \<lbrace> X \<longmapsto> Y\<^sub>F \<^bold>t\<^bold>h\<^bold>r\<^bold>o\<^bold>w\<^bold>s E\<^sub>F \<rbrace>)
+\<Longrightarrow> (\<And>v. \<^bold>v\<^bold>i\<^bold>e\<^bold>w If C (Y\<^sub>T v) (Y\<^sub>F v) \<longmapsto> Y v \<^bold><\<^bold>a\<^bold>c\<^bold>t\<^bold>i\<^bold>o\<^bold>n\<^bold>> branch_convergence)
+\<Longrightarrow> \<^bold>p\<^bold>r\<^bold>o\<^bold>c op_if br\<^sub>T br\<^sub>F rawc \<lbrace> X\<heavy_comma> C \<Ztypecolon> \<^bold>v\<^bold>a\<^bold>l[rawc] \<bool> \<longmapsto> Y \<^bold>t\<^bold>h\<^bold>r\<^bold>o\<^bold>w\<^bold>s \<lambda>e. (E\<^sub>T e \<^bold>s\<^bold>u\<^bold>b\<^bold>j C) + (E\<^sub>F e \<^bold>s\<^bold>u\<^bold>b\<^bold>j \<not> C) \<rbrace>\<close>
+  unfolding op_if_def Premise_def Action_Tag_def
+  apply (cases rawc; cases C; simp; rule; simp add: \<phi>expns WT_bool)
+  using \<phi>CONSEQ view_shift_id by blast+
+
+proc "if":
+  assumes C: \<open>\<^bold>p\<^bold>r\<^bold>o\<^bold>c cond \<lbrace> X \<longmapsto> X1\<heavy_comma> \<^bold>v\<^bold>a\<^bold>l C \<Ztypecolon> \<bool> \<^bold>t\<^bold>h\<^bold>r\<^bold>o\<^bold>w\<^bold>s E \<rbrace>\<close>
+      and brT: \<open>\<^bold>p\<^bold>r\<^bold>e\<^bold>m\<^bold>i\<^bold>s\<^bold>e   C \<longrightarrow> \<^bold>p\<^bold>r\<^bold>o\<^bold>c brT \<lbrace> X1 \<longmapsto> Y\<^sub>T (ret::'a sem_value) \<^bold>t\<^bold>h\<^bold>r\<^bold>o\<^bold>w\<^bold>s E\<^sub>T \<rbrace>\<close>
+      and brF: \<open>\<^bold>p\<^bold>r\<^bold>e\<^bold>m\<^bold>i\<^bold>s\<^bold>e \<not> C \<longrightarrow> \<^bold>p\<^bold>r\<^bold>o\<^bold>c brF \<lbrace> X1 \<longmapsto> Y\<^sub>F (ret::'a sem_value) \<^bold>t\<^bold>h\<^bold>r\<^bold>o\<^bold>w\<^bold>s E\<^sub>F \<rbrace>\<close>
+      and [\<phi>reason 9999 for \<open>\<^bold>v\<^bold>i\<^bold>e\<^bold>w If C (Y\<^sub>T ?v) (Y\<^sub>F ?v) \<longmapsto> ?Y \<^bold><\<^bold>a\<^bold>c\<^bold>t\<^bold>i\<^bold>o\<^bold>n\<^bold>> branch_convergence\<close>]:
+              \<open>(\<And>v. \<^bold>v\<^bold>i\<^bold>e\<^bold>w If C (Y\<^sub>T v) (Y\<^sub>F v) \<longmapsto> Y v \<^bold><\<^bold>a\<^bold>c\<^bold>t\<^bold>i\<^bold>o\<^bold>n\<^bold>> branch_convergence)\<close>
+  argument \<open>X\<close>
+  return \<open>Y (ret::'a sem_value)\<close>
+  throws \<open>\<lambda>e. E e + (E\<^sub>T e \<^bold>s\<^bold>u\<^bold>b\<^bold>j C) + (E\<^sub>F e \<^bold>s\<^bold>u\<^bold>b\<^bold>j \<not> C)\<close>
+  \<medium_left_bracket> C branch brT brF \<medium_right_bracket>. .
+
+subsection \<open>Loops\<close>
+
+lemma "__DoWhile__rule_\<phi>app":
+  " \<^bold>p\<^bold>r\<^bold>o\<^bold>c body \<lbrace> X x \<^bold>s\<^bold>u\<^bold>b\<^bold>j x. P x \<longmapsto> (\<exists>*x'. X x' \<heavy_comma> \<^bold>v\<^bold>a\<^bold>l P x' \<Ztypecolon> \<bool>) \<^bold>t\<^bold>h\<^bold>r\<^bold>o\<^bold>w\<^bold>s E\<rbrace>
+\<Longrightarrow> \<^bold>p\<^bold>r\<^bold>o\<^bold>c op_do_while body \<lbrace> X x \<^bold>s\<^bold>u\<^bold>b\<^bold>j x. P x \<longmapsto> X x' \<^bold>s\<^bold>u\<^bold>b\<^bold>j x'. \<not> P x' \<^bold>t\<^bold>h\<^bold>r\<^bold>o\<^bold>w\<^bold>s E \<rbrace>"
+  unfolding op_do_while_def \<phi>Procedure_def
+  apply (simp add: subset_iff LooseStateTy_expn')
+  apply (rule allI impI conjI)+
+  subgoal for comp R s
+  apply (rotate_tac 2)
+    apply (induct body comp s rule: SemDoWhile.induct; clarsimp simp add: \<phi>expns times_list_def)
+    apply fastforce
+    subgoal premises prems for res f s s'' c u v proof -
+      have t1: \<open>\<exists>c. (\<exists>fic. (\<exists>u v. fic = u * v \<and> u \<in> R \<and> v \<in> X c \<and> u ## v) \<and> s \<in> INTERP_RES fic) \<and> P c\<close>
+        using prems(5) prems(6) prems(7) prems(8) prems(9) by blast
+      show ?thesis
+        apply (insert \<open>\<forall>_ _. (\<exists>_. _) \<longrightarrow> _\<close>[THEN spec[where x=s], THEN spec[where x=R], THEN mp, OF t1])
+        using prems(1) prems(3) by fastforce
+    qed
+    apply fastforce
+    by blast .
+
+lemma
+  " \<^bold>p\<^bold>r\<^bold>o\<^bold>c body \<lbrace> X x \<^bold>s\<^bold>u\<^bold>b\<^bold>j x. I x \<and> P x \<longmapsto> X x' \<heavy_comma> \<^bold>v\<^bold>a\<^bold>l P x' \<Ztypecolon> \<bool> \<^bold>s\<^bold>u\<^bold>b\<^bold>j x'. I x' \<^bold>t\<^bold>h\<^bold>r\<^bold>o\<^bold>w\<^bold>s \<lambda>e. E e x' \<^bold>s\<^bold>u\<^bold>b\<^bold>j x'. I x'\<rbrace>
+\<Longrightarrow> \<^bold>p\<^bold>r\<^bold>o\<^bold>c op_do_while body \<lbrace> X x \<^bold>s\<^bold>u\<^bold>b\<^bold>j x. I x \<and> P x \<longmapsto> X x' \<^bold>s\<^bold>u\<^bold>b\<^bold>j x'. I x' \<and> \<not> P x' \<^bold>t\<^bold>h\<^bold>r\<^bold>o\<^bold>w\<^bold>s \<lambda>e. E e x' \<^bold>s\<^bold>u\<^bold>b\<^bold>j x'. I x' \<rbrace>"
+  using "__DoWhile__rule_\<phi>app"[where X=\<open>\<lambda>x. X x \<^bold>s\<^bold>u\<^bold>b\<^bold>j I x\<close> and P=P,
+            simplified Subjection_times, simplified] .
+
+proc (nodef) do_while:
+assumes \<open>\<^bold>p\<^bold>a\<^bold>r\<^bold>a\<^bold>m ( X' x \<^bold>s\<^bold>u\<^bold>b\<^bold>j x. Inv: invariant x \<and> Guard: cond x)\<close>
+    and V: \<open>\<^bold>v\<^bold>i\<^bold>e\<^bold>w X \<longmapsto> ( X' x \<^bold>s\<^bold>u\<^bold>b\<^bold>j x. invariant x \<and> cond x) \<^bold>w\<^bold>i\<^bold>t\<^bold>h Any \<^bold><\<^bold>a\<^bold>c\<^bold>t\<^bold>i\<^bold>o\<^bold>n\<^bold>> ToSA\<close>
+assumes B: \<open>\<forall>x. \<^bold>p\<^bold>r\<^bold>e\<^bold>m\<^bold>i\<^bold>s\<^bold>e cond x \<longrightarrow> \<^bold>p\<^bold>r\<^bold>e\<^bold>m\<^bold>i\<^bold>s\<^bold>e invariant x
+    \<longrightarrow> \<^bold>p\<^bold>r\<^bold>o\<^bold>c body \<lbrace> X' x \<longmapsto> (X' x'\<heavy_comma> \<^bold>v\<^bold>a\<^bold>l cond x' \<Ztypecolon> \<bool> \<^bold>s\<^bold>u\<^bold>b\<^bold>j x'. invariant x') \<^bold>t\<^bold>h\<^bold>r\<^bold>o\<^bold>w\<^bold>s E \<rbrace>\<close>
+argument \<open>X\<close>
+return   \<open>X' x' \<^bold>s\<^bold>u\<^bold>b\<^bold>j x'. invariant x' \<and> \<not> cond x'\<close>
+throws E
+  \<medium_left_bracket>
+  V[unfolded Action_Tag_def]
+  "__DoWhile__rule_\<phi>app"[where P=cond and X=\<open>\<lambda>x'. X' x' \<^bold>s\<^bold>u\<^bold>b\<^bold>j invariant x'\<close>, simplified]
+  \<medium_left_bracket> B \<medium_right_bracket>.
+  \<medium_right_bracket> by simp .
+
+proc while:
+  assumes \<open>\<^bold>p\<^bold>a\<^bold>r\<^bold>a\<^bold>m ( X x \<^bold>s\<^bold>u\<^bold>b\<^bold>j x. Inv: invariant x \<and> Guard: cond x)\<close>
+  assumes V[unfolded Action_Tag_def]:
+           "\<^bold>v\<^bold>i\<^bold>e\<^bold>w X' \<longmapsto> (X x \<^bold>s\<^bold>u\<^bold>b\<^bold>j x. invariant x) \<^bold>w\<^bold>i\<^bold>t\<^bold>h Any \<^bold><\<^bold>a\<^bold>c\<^bold>t\<^bold>i\<^bold>o\<^bold>n\<^bold>> ToSA"
+    and C: "\<forall>x. \<^bold>p\<^bold>r\<^bold>e\<^bold>m\<^bold>i\<^bold>s\<^bold>e invariant x \<longrightarrow> \<^bold>p\<^bold>r\<^bold>o\<^bold>c Cond \<lbrace> X x \<longmapsto> X x'\<heavy_comma> \<^bold>v\<^bold>a\<^bold>l cond x' \<Ztypecolon> \<bool> \<^bold>s\<^bold>u\<^bold>b\<^bold>j x'. invariant x' \<rbrace>"
+    and B: "\<forall>x. \<^bold>p\<^bold>r\<^bold>e\<^bold>m\<^bold>i\<^bold>s\<^bold>e invariant x \<longrightarrow> \<^bold>p\<^bold>r\<^bold>e\<^bold>m\<^bold>i\<^bold>s\<^bold>e cond x \<longrightarrow> \<^bold>p\<^bold>r\<^bold>o\<^bold>c Body \<lbrace> X x \<longmapsto> X x' \<^bold>s\<^bold>u\<^bold>b\<^bold>j x'. invariant x' \<rbrace>"
+  argument \<open>X'\<close>
+  return \<open>X x \<^bold>s\<^bold>u\<^bold>b\<^bold>j x. invariant x \<and> \<not> cond x\<close>
+  \<medium_left_bracket> V C
+    branch \<medium_left_bracket>
+      do_while \<open>X vars \<^bold>s\<^bold>u\<^bold>b\<^bold>j vars. Inv: invariant vars \<and> Guard: cond vars\<close>
+      \<medium_left_bracket> B C \<medium_right_bracket>.
+      \<medium_right_bracket>.
+    \<medium_left_bracket> \<medium_right_bracket> for \<open>X vars \<^bold>s\<^bold>u\<^bold>b\<^bold>j vars. invariant vars \<and> \<not> cond vars\<close> ..
+  \<medium_right_bracket>. .
+
+(*
+We fail to infer the abstract loop guard automatically but require users to give.
+The main problem is about nondeterminancy in higher-order unification.
+In the below rule, in \<^term>\<open>cond x' \<Ztypecolon> \<bool>\<close>, both \<open>cond\<close> and \<open>x'\<close> are schematic variables,
+which means we cannot determine either of them via unification.
+Even though the abstract state \<open>x'\<close> may be determined possibly in the unification of \<open>X x'\<close>,
+to infer \<open>cond x'\<close> it is still a problem especially when \<open>x'\<close> is not a variable but a composite
+term and its composite expression may be shattered in the expression of \<open>cond\<close> after
+rewrites and simplifications, causing it is very difficult to recover the actual abstract guard
+\<open>cond\<close> from simplified composition \<open>cond x'\<close>.
+*)
+
+end
