Phi_Semantics/PhiSem_Machine_Integer_Boolean.thy
@@ -1,0 +1,14 @@
+theory PhiSem_Machine_Integer_Boolean
+  imports PhiSem_Machine_Integer
+begin
+
+specification (bool) bool_def'[discharging_semantic_debt]:
+  \<open>bool = int 1\<close> by blast
+
+specification (V_bool) V_bool_def'[discharging_semantic_debt]:
+    \<open>V_bool = lift_Field (\<lambda>(_,x). x = 1) (\<lambda>b. (1, if b then 1 else 0)) V_int\<close>
+  by blast
+
+hide_fact bool_def V_bool_def
+
+end
